doc, refactor

src/Internal/WfTuples.v
@@ -4,8 +4,7 @@ Require Import Coq.Lists.List.
 Require Import Coq.Sorting.Permutation.
 Require Import Relation_Definitions.
 Require Import Relation_Operators.
-From Coq.Wellfounded
-  Require Import Inclusion Inverse_Image Transitive_Closure.
+From Coq.Wellfounded Require Import Inclusion Inverse_Image Transitive_Closure.
 Add LoadPath "src".
 From Internal Require Wff2.
 (* end hide *)
@@ -43,6 +42,13 @@ Variable lt: A -> A -> Prop.
 Variable wf_lt: well_founded lt.
 Local Infix "<" := lt.
 
+Definition lltlp := (clos_trans _ (Wff2.ltlp lt)).
+Definition wf_trans: well_founded lltlp.
+Proof.
+  apply wf_clos_trans. apply Wff2.wf_perm. apply wf_lt.
+Qed.
+
+
 (** 2 *)
 
 Definition le12 : A -> A * A -> Prop := fun a bs =>
@@ -53,21 +59,13 @@ Definition le22 : A * A -> A * A -> Prop := fun a bs =>
 Local Infix "<<" := le22 (at level 50).
 
 Definition list2 {A: Type} := fun x: prod A A => let (x1, x2) := x in 
-  cons x1 (cons x2 nil).
-
-  
-Definition permletrans := (clos_trans _ (Wff2.permle lt)).
-Definition wf_trans: well_founded permletrans.
-Proof.
-  apply wf_clos_trans. apply Wff2.wf_perm. apply wf_lt.
-Qed.
-
+  x1 :: x2 :: nil.
 
 Lemma le2lst:
-  forall x y, x << y -> permletrans (list2 x) (list2 y).
+  forall x y, x << y -> lltlp (list2 x) (list2 y).
 Proof.
   intros. destruct x, y. destruct H, H, H0; simpl list2.
-   - apply (t_trans _ _ _ (cons a1 nil)); apply t_step.
+   - apply (t_trans _ _ _ (a1 :: nil)); apply t_step.
      red. exists (a :: a0 :: nil). split; auto. 
      pose proof (Wff2.C _ lt O (a1 :: nil) (a :: a0 :: nil) ). simpl in H1. auto.
      exists (a1 :: nil). split; auto. 
@@ -91,9 +89,9 @@ Qed.
 
 Theorem wf_two: well_founded le22.
 Proof.
-  apply (wf_incl _ _ (fun x y => permletrans (list2 x) (list2 y))).
+  apply (wf_incl _ _ (fun x y => lltlp (list2 x) (list2 y))).
   unfold inclusion. apply le2lst.
-  apply (wf_inverse_image _ _ (permletrans) list2).
+  apply (wf_inverse_image _ _ (lltlp) list2).
   apply wf_clos_trans.
   apply Wff2.wf_perm.
   apply wf_lt.
@@ -126,10 +124,10 @@ Definition list3 {A: Type} := fun x : A *A *A=>
   x1 :: x2 :: x3 :: nil end.
 
 Lemma le3lst:
-  forall x y, x <<< y -> permletrans (list3 x) (list3 y).
+  forall x y, x <<< y -> lltlp (list3 x) (list3 y).
 Proof.
   intros. destruct x, y, p, p0. destruct H, H, H0, H0, H1; simpl list3.
-  - apply (t_trans _ _ _ (cons a3 nil)).
+  - apply (t_trans _ _ _ (a3 :: nil)).
   -- apply t_step. red. exists (a1 :: a2 :: a :: nil). split. 
     reflexivity.
     pose proof (Wff2.C _ lt O (a3 :: nil) (a1 :: a2 :: a :: nil) ). simpl in H2. auto.
@@ -143,9 +141,9 @@ Admitted.
 
 Theorem wf_three: well_founded le33.
 Proof.
-  apply (wf_incl _ _ (fun x y => permletrans (list3 x) (list3 y))).
+  apply (wf_incl _ _ (fun x y => lltlp (list3 x) (list3 y))).
   unfold inclusion. apply le3lst.
-  apply (wf_inverse_image _ _ (permletrans) list3).
+  apply (wf_inverse_image _ _ (lltlp) list3).
   apply wf_clos_trans.
   apply Wff2.wf_perm.
   apply wf_lt.
@@ -165,6 +163,53 @@ Proof.
     apply (H0 (y1, y2, y3)). assumption.
 Qed.
 
+(* N *)
+(* 
+Fixpoint tupleN n : Type := match n with
+  | O => A
+  | S m => prod A (tupleN m)
+  end.
+
+Fixpoint le1M {m} : A -> tupleN m -> Prop :=
+  match m with 
+  | O => lt
+  | S _ => fun a t => let (a', t') := t in a < a' /\ le1M a t'
+  end.
+
+Fixpoint leNM {n m} : tupleN n -> tupleN m -> Prop :=
+  match n with 
+  | O => le1M
+  | S _ => fun t s => let (a, t') := t in le1M a s /\ leNM t' s
+  end.
+
+  (* Continue here *)
+Definition listN {n} : tupleN n -> list A := match n with
+
+Lemma le2lst:
+  forall x y, x << y -> lltlp (list2 x) (list2 y).
+Proof.
+  intros. destruct x, y. destruct H, H, H0; simpl list2.
+   - apply (t_trans _ _ _ (a1 :: nil)); apply t_step.
+     red. exists (a :: a0 :: nil). split; auto. 
+     pose proof (Wff2.C _ lt O (a1 :: nil) (a :: a0 :: nil) ). simpl in H1. auto.
+     exists (a1 :: nil). split; auto. 
+     pose proof (Wff2.C _ lt 1 (a1 :: a2 :: nil) nil). simpl in H1. auto.
+  - apply (t_trans _ _ _ (a1 :: a0 :: nil)); apply t_step.
+    red. exists (a :: a0 :: nil). split; auto. 
+    pose proof (Wff2.C _ lt O (a1 :: a0 :: nil) (a :: nil) ). simpl in H1. auto.
+    exists (a1 :: a0 :: nil). split; auto. 
+    pose proof (Wff2.C _ lt 1 (a1 :: a2 :: nil) (a0 :: nil)). simpl in H1. auto.
+  - apply (t_trans _ _ _ (a0 :: a2 :: nil)); apply t_step.
+    red. exists (a0 :: a :: nil). split. apply perm_swap.
+    pose proof (Wff2.C _ lt 1 (a0 :: a2 :: nil) (a :: nil)). simpl in H1. auto.
+    exists (a0 :: a2 :: nil). split; auto. 
+    pose proof (Wff2.C _ lt O (a1 :: a2 :: nil) (a0 :: nil) ). simpl in H1. auto.
+  - apply (t_trans _ _ _ (a2 :: nil)); apply t_step.
+    red. exists (a :: a0 :: nil). split; auto. 
+    pose proof (Wff2.C _ lt O (a2 :: nil) (a :: a0 :: nil) ). simpl in H1. auto.
+    exists (a2 :: nil). split; auto. 
+    pose proof (Wff2.C _ lt 0 (a1 :: a2 :: nil) nil). simpl in H1. auto.
+Qed. *)
 
 End MultiWf.
 
