src/Internal/Wff2.v
@@ -12,11 +12,11 @@ Require Import Coq.Program.Equality.
 Require Import Coq.omega.Omega.
 Require Import Coq.Sorting.Permutation.
 
-
 Section Wff2.
 
 Variable A : Type.
 Variable lt : A -> A -> Prop.
+Local Infix "<<" := lt (at level 80).
 Variable wf_lt: well_founded lt.
 
 (** Replace an element of a list by concatenating another list in its place: *)
@@ -30,14 +30,14 @@ Proof.
   - intros. refine (a :: IHi l (lt_S_n _ _ H) X).
 Defined.
 
-Lemma replace_succ: forall {i l l' x} (p: S i < length (x::l)) (p': i < length l),
+Lemma replace_cons: forall {i x l l'} (p: S i < length (x::l)) (p': i < length l),
   replace p l' = x :: replace p' l'.
 Proof.
   induction i; intros; destruct l; simpl length in *.
   - omega.
   - reflexivity.
   - omega.
-  - simpl. setoid_rewrite (IHi l l' a). apply eq_refl.
+  - simpl. setoid_rewrite (IHi a l l'). apply eq_refl.
   Grab Existential Variables. apply (lt_S_n _ _ p').
 Qed.
 
@@ -51,7 +51,7 @@ Proof.
   - intros. refine (IHi l (lt_S_n _ _ H)).
 Defined.
 
-Lemma get_succ: forall {i x l} (p: S i < length (x::l)) (p': i < length (l)),
+Lemma get_cons: forall {i x l} (p: S i < length (x::l)) (p': i < length (l)),
   get p = get p'.
 Proof.
   induction i; intros; destruct l; simpl length in *.
@@ -69,30 +69,39 @@ Fixpoint all P (l: list A) := match l with
 end.
 
 (* rename to ltl *)
-Inductive lt_lst : list A -> list A -> Prop :=
+Inductive ltl : list A -> list A -> Prop :=
   | C : forall i (l l': list A) (p: i < length l),
          all (fun x => lt x (get p)) l'
-          -> lt_lst (replace p l') l .
+          -> ltl (replace p l') l .
+Local Infix "<<<" := ltl (at level 80).
 
+(** A useful inversion lemma.  *)
 Lemma ltl_cases: forall {y a l}, 
-  lt_lst y (a :: l) -> 
-    (exists l', lt_lst l' l /\ y = a :: l') \/
-      (exists l', y = l' ++ l /\ all (fun x => lt x a) l').
+  y <<< a::l
+    -> (exists l', l' <<< l /\ y = a :: l')
+      \/ exists l', y = l' ++ l /\ all (fun x => lt x a) l'.
 Proof.
   intros. dependent destruction H.
   induction i.
   - right. exists l'. simpl. split; auto.
   - left. exists (replace (lt_S_n _ _ p) l'). split.
-    pose proof (get_succ p).
+    pose proof (get_cons p).
     refine (C _ l l' (lt_S_n _ _ p) H).
-    apply (replace_succ p).
+    apply (replace_cons p).
 Qed.
 
+(** We follow the proof of wellfoundedness of the multiset
+    order in by Tobias Nipkov in "An inductive Proof of the 
+    Wellfoundedness of the Multiset Order". We adapt the lemmas
+    in that document to the case of lists instead of multisets.
+*)
+
+(** Lemma 2.1 *)
 Lemma l2p1: forall {a M0},
-  (forall b, lt b a -> forall M, Acc lt_lst M -> Acc lt_lst (b :: M))
-  -> Acc lt_lst M0
-  -> (forall M, lt_lst M M0 -> Acc lt_lst (a :: M))
-  -> Acc lt_lst (a :: M0).
+  (forall b, b << a -> forall M, Acc ltl M -> Acc ltl (b :: M))
+    -> Acc ltl M0
+      -> (forall M, M <<< M0 -> Acc ltl (a :: M))
+        -> Acc ltl (a :: M0).
 Proof.
   intros. apply Acc_intro. intros. destruct (ltl_cases H2).
   - destruct H3, H3. rewrite H4 in *. clear H4 y. apply (H1 x H3).
@@ -102,29 +111,30 @@ Proof.
       apply (C O (a :: M0) x (Nat.lt_0_succ _) H4).
 Qed.
 
-Lemma l2p2: forall x,
-(forall y : A, lt y x -> forall M, Acc lt_lst M -> Acc lt_lst (y :: M))
--> forall M, (Acc lt_lst M) ->  Acc lt_lst (x :: M).
+(** Lemma 2.2 *)
+Lemma l2p2: forall a,
+  (forall b, b << a -> forall M, Acc ltl M -> Acc ltl (b :: M))
+    -> forall M, Acc ltl M ->  Acc ltl (a :: M).
 Proof.
   intros.
-    refine (@Fix_F (list A) lt_lst (fun M0 => Acc lt_lst M0 -> Acc lt_lst (x::M0)) _ M H0 H0). intros.
-    rename x0 into M0.
+    refine (@Fix_F (list A) ltl (fun M0 => Acc ltl M0 -> Acc ltl (a::M0)) _ M H0 H0). intros M0 H1 H2.
     pose H2 as H2'. destruct H2'. pose proof (fun y h => H1 y h (H3 y h)).
     revert H H2 H4. clear. exact l2p1.
 Qed.
 
-Lemma l2p3: forall {M} a, Acc lt_lst M -> Acc lt_lst (cons a M).
+(** Lemma 2.3 *)
+Lemma l2p3: forall {a} M, Acc ltl M -> Acc ltl (a :: M).
 Proof.
-  intros M a. revert M. apply (well_founded_ind wf_lt (fun a => forall M, Acc lt_lst M -> Acc lt_lst (cons a M))).
+  apply (well_founded_ind wf_lt (fun a => forall M, Acc ltl M -> Acc ltl (a :: M))).
   exact l2p2. 
 Qed.
 
-Theorem wf_lst: well_founded lt_lst.
+Theorem wf_ltl: well_founded ltl.
 Proof.
   unfold well_founded. intro l. induction l.
   - apply Acc_intro. intros. dependent destruction H.
     simpl length in p. omega.
-  - apply (l2p3 a IHl).
+  - apply (l2p3 l IHl).
 Qed.
 
 (** * Unordered
@@ -135,20 +145,19 @@ Qed.
     (see https://coq.github.io/doc/master/stdlib/Coq.Sorting.Permutation.html).
 *)
 
-(* Rename to ltlp ? *)
-Definition permle l l' := exists l'', Permutation l l'' /\ lt_lst l'' l'.
+Definition ltlp l l' := exists l'', Permutation l l'' /\ l'' <<< l'.
 
-Lemma perm_lt_dx: forall {a b b'}, Permutation b b' -> lt_lst a b' -> permle a b.
+Lemma perm_lt_dx: forall {a b b'}, Permutation b b' -> a <<< b' -> ltlp a b.
 Proof.
-  intros. revert a H0. dependent induction H; intros; unfold permle.
+  intros. revert a H0. dependent induction H; intros; unfold ltlp.
   - dependent destruction H0. simpl length in p. omega.
   - destruct (ltl_cases H0); destruct H1, H1.
   -- rewrite H2 in *. clear a H2.
     destruct (IHPermutation _ H1), H2.
     exists (x :: x1). split.
   --- apply perm_skip. auto.
-  --- dependent destruction H3. rewrite<- (replace_succ (lt_n_S _ _ p)).
-      refine (C (S i) (x::l) l'0 _ _). rewrite (get_succ _ p). auto.
+  --- dependent destruction H3. rewrite<- (replace_cons (lt_n_S _ _ p)).
+      refine (C (S i) (x::l) l'0 _ _). rewrite (get_cons _ p). auto.
   -- rewrite H1 in *. clear a H1. exists (x0 ++ l). split.
      apply Permutation_app_head. apply Permutation_sym. auto.
      refine (C O (x::l) x0 _ H2). simpl length. omega.
@@ -159,10 +168,10 @@ Proof.
       dependent destruction H1.
       pose proof ((lt_n_S _ _ (lt_n_S _ _ p)) : S (S i) < length (y :: x :: l)).
       pose proof (fun X => C (S (S i)) (y :: x :: l) l' H2 X). simpl replace in H3.
-      setoid_rewrite replace_succ in H3. apply H3.
+      setoid_rewrite replace_cons in H3. apply H3.
       cut (get H2 = get p). intro. rewrite H4. assumption.
       simpl get.
-      setoid_rewrite get_succ. apply eq_refl. auto.
+      setoid_rewrite get_cons. apply eq_refl. auto.
   --- rewrite H1 in *. clear x0 H1. exists (x1 ++ x :: l). split.
       apply Permutation_cons_app. reflexivity.
       refine (C O (y :: x :: l) x1 _ _). apply H2.
@@ -174,25 +183,25 @@ Proof.
     Grab Existential Variables. simpl length. omega. simpl length. omega.
 Qed.
 
-Lemma perm_Acc : forall l l', Permutation l l' -> Acc permle l -> Acc permle l'.
+Lemma perm_Acc : forall l l', Permutation l l' -> Acc ltlp l -> Acc ltlp l'.
 Proof.
   intros. induction H.
   - auto.
-  - apply Acc_intro. intros. apply H0. destruct H1, H1. unfold permle.
+  - apply Acc_intro. intros. apply H0. destruct H1, H1. unfold ltlp.
     destruct (perm_lt_dx (perm_skip x H) H2). destruct H3. exists x1. split.
     transitivity x0; auto. auto.
-  - apply Acc_intro. intros. apply H0. destruct H, H. unfold permle.
+  - apply Acc_intro. intros. apply H0. destruct H, H. unfold ltlp.
     destruct (perm_lt_dx (perm_swap x y l) H1). destruct H2. exists x1. split.
     transitivity x0; auto. auto.
   - auto.
 Qed.
 
-Theorem wf_perm : well_founded permle.
+Theorem wf_perm : well_founded ltlp.
 Proof.
-    intro a. induction (wf_lst a). apply Acc_intro. intros.
+    intro a. induction (wf_ltl a). apply Acc_intro. intros.
     destruct H1, H1. apply (perm_Acc _ _ (Permutation_sym H1)). auto.
 Qed.
 End Wff2.
 
-Arguments permle : default implicits.
+Arguments ltlp : default implicits.
 Arguments wf_perm : default implicits.
